@prefix rdf:  <http://www.w3.org/1999/02/22-rdf-syntax-ns#>.
@prefix rdfs: <http://www.w3.org/2000/01/rdf-schema#>.
@prefix xsd: <http://www.w3.org/2001/XMLSchema#>.
@prefix : <http://spd.ivl.cns/cim/rtdbmof#>.

 :id a rdf:Property ;
    rdfs:range xsd:string ;
    rdfs:label "RTDB ID"@ru ;
    rdfs:label "RTDB ID"@en ;
    rdfs:comment "Идентификатор RTDB"@ru ;
    rdfs:comment "Identifier RTDB"@en .

 :alert_hysteresis a rdf:Property ;
    rdfs:label "Гистерезис оповещения"@ru ;
    rdfs:label "Alert hysteresis"@en ;
    rdfs:range xsd:int .

 :typecode a rdf:Property ;
    rdfs:domain :Array ;
    rdfs:range xsd:string ;
    rdfs:label "Тип"@ru ;
    rdfs:comment "Код типа массива"@ru .

 :arr_IO a rdf:Property ;
    rdfs:domain :Array ;
    rdfs:range xsd:string ;
    rdfs:label "I/O"@ru ;
    rdfs:comment "Код функции I/O массива"@ru .

 :tick a rdf:Property ;
    rdfs:domain :Array ;
    rdfs:range xsd:unsignedInt ;
    rdfs:label "Частота обновления"@ru ;
    rdfs:comment "Предполагаемая частота обновления массива в секундах. 0 - частота не определена"@ru .

 :arr_size a rdf:Property ;
    rdfs:domain :Array ;
    rdfs:range xsd:int ;
    rdfs:label "Размер массива"@ru ;
    rdfs:comment "Размер массива"@ru .

 :PPClass a rdfs:Class ;
    rdfs:label "Тэг класс"@ru .

 :ProcessPoint a :PPClass ;
    rdfs:label "Тэг"@ru .

 :Discrete a :PPClass ;
   rdfs:subClassOf :ProcessPoint ;
   rdfs:label "Дискретный параметр"@ru .

 :Analog  a :PPClass ;
   rdfs:subClassOf :ProcessPoint;
   rdfs:label "Аналоговый параметр"@ru ;
   rdfs:comment "Аналоговый параметр"@ru .

 :format a rdf:Property ;
    rdfs:domain :Analog ;
    rdfs:label "FORMAT"@en ;
    rdfs:label "Формат вывода"@ru ;
    rdfs:comment """
Заполняется в виде M.N, где
M – общее количество знаков включая точку и знак ( не более 7);
N – количество знаков после запятой.
Научный формат определяется в виде NE, где
N – общее количество знаков мантиссы, включая точку и знак, ( если он есть).
Определяет формат  для отображения параметров на РМО и в протоколах регистрации.
При задании научного формата число представляется в виде стандартно нормализованного числа и соответствующей ему степени  N,NNNE-XX"""@ru .

 :array a rdf:Property ;
    rdfs:domain :ProcessPoint ;
    rdfs:range :Array ;
    rdfs:label "Массив"@ru ;
    rdfs:label "Array"@en ;
    rdfs:comment "RTDB массив, в котором находится динамические значения элемента"@ru ;
    rdfs:comment "RTDB array, which contains the dynamic values of the element"@en .

 :arr_index a rdf:Property ;
    rdfs:domain :ProcessPoint ;
    rdfs:range xsd:int ;
    rdfs:label "Индекс"@ru ;
    rdfs:label "Index"@en ;
    rdfs:comment "Индекс элемента в массиве RTDB"@ru ;
    rdfs:comment "The index of the element in the RTDB array"@en .

 :title a rdf:Property ;
    rdfs:domain :ProcessPoint ;
    rdfs:range xsd:string ;
    rdfs:label "Title"@en ; 
    rdfs:label "Наименование"@ru ; 
    rdfs:comment "Item Description"@en ; 
    rdfs:comment "Наименование объекта"@ru ; 
    :opc-id 101 .

 :mu a  rdf:Property ;
    rdfs:domain :Analog ;
    rdfs:label "EU Units"@en ; 
    rdfs:label "Ед.изм."@ru ; 
    rdfs:comment "Единица измерения"@ru ; 
    rdfs:comment "Unit of measurement"@en ; 
    :opc-id 100 .

 :HIR   a rdf:Property ;
    rdfs:domain :Analog ;
    rdfs:range xsd:float ;
    rdfs:label "High Instr.Range"@en ; 
    rdfs:label "Верх.предел измер."@ru ;
    rdfs:comment "Верхний предел измерения"@ru ;
    rdfs:comment """OPC: High Instrument Range. This represents the highest value that 
can be returned by the instrument."""@en ; 
    :opc-id 104 .

 :LIR   a rdf:Property ;
    rdfs:domain :Analog ;
    rdfs:range xsd:float ;
    rdfs:label "Low Instr.Range"@en ; 
    rdfs:label "Нижн.предел измер."@ru ; 
    rdfs:comment "Нижний предел измерения"@ru ; 
    rdfs:comment """OPC: Low Instrument Range. This represents the lowest value that 
can be returned by the instrument."""@en ; 
    :opc-id 105 .

 :HEU a rdf:Property ;
    rdfs:domain :Analog ;
    rdfs:range xsd:float ;
    rdfs:label "High EU"@en ; 
    rdfs:label "Верхний предел физ.д-на"@ru ;
    rdfs:comment "Верхний предел физического диапазона"@ru ;
    rdfs:comment """OPC: Present only for analog data. This represents the highest value likely 
to be obtained in normal operation and is intended for such use as 
automatically scaling a bargraph display. 
"""@en ; 
    :opc-id 102 .

 :LEU   a rdf:Property ;
    rdfs:domain :Analog ;
    rdfs:range xsd:float ;
    rdfs:label "Low EU"@en ; 
    rdfs:label "Нижний предел физ.д-на"@ru ; 
    rdfs:comment "Нижний предел физического диапазона"@ru ; 
    rdfs:comment """OPC: Present only for analog data. This represents the lowest value likely 
to be obtained in normal operation and is intended for such use as 
automatically scaling a bargraph display. 
"""@en ; 
    :opc-id 103 .

 :State a rdf:Property ;
    rdfs:domain :ProcessPoint ;
    rdfs:range xsd:string ;
    rdfs:label "Condition Status"@en ; 
    rdfs:comment """OPC: The current alarm or condition status associated with the Item 
e.g. "NORMAL", "ACTIVE", "HI ALARM", etc  
"""@en ; 
    :opc-id 300 .

 :Deadband a rdf:Property ;
    rdfs:domain :Analog ;
    rdfs:range xsd:float ;
    rdfs:label "Deadband"@en ; 
    :opc-id 306 .

 :HHL   a rdf:Property ;
    rdfs:domain :Analog ;
    rdfs:range xsd:float ;
    rdfs:label "HiHi Limit"@en ; 
    rdfs:label "ВАГ"@ru ; 
    rdfs:comment "Верхняя аварийная граница"@ru ; 
    rdfs:comment """OPC: Each Tag has a High High Limit Parameter which acts as 
the Tag's High High Alarm Limit for evaluating alarm conditions from the Value Parameter.  
If the value of the Value Parameter exceeds the High High Limit the Tag is considered 
to be in a High High alarm condition."""@en ; 
    :opc-id 307 .

 :HL    a rdf:Property ;
    rdfs:domain :Analog ;
    rdfs:range xsd:float ;
    rdfs:label "Hi Limit"@en ; 
    rdfs:label "ВРГ"@ru ; 
    rdfs:comment "Верхняя граница регламентного диапазона"@ru ; 
    rdfs:comment """OPC: Each Tag has a High Limit Parameter which acts as 
the Tag's High Alarm Limit for evaluating alarm conditions from the Value Parameter.  
If the value of the Value Parameter exceeds the High Limit the Tag is considered 
to be in a High alarm condition."""@en ; 
    :opc-id 308 .

 :LL    a rdf:Property ;
    rdfs:domain :Analog ;
    rdfs:range xsd:float ;
    rdfs:label "Lo Limit"@en ; 
    rdfs:label "НРГ"@ru ; 
    rdfs:comment "Нижняя граница регламентного диапазона"@ru ; 
    rdfs:comment """OPC: Each Tag has a Low Limit Parameter which acts as 
the Tag's Low Alarm Limit for evaluating alarm conditions from the Value Parameter.  
If the value of the Value Parameter exceeds the Low Limit the Tag is considered 
to be in a Low alarm condition."""@en ; 
    :opc-id 309 .

 :LLL   a rdf:Property ;
    rdfs:domain :Analog ;
    rdfs:range xsd:float ;
    rdfs:label "LoLo Limit"@en ; 
    rdfs:label "НАГ"@ru ; 
    rdfs:comment "Нижняя аварийная граница"@ru ; 
    rdfs:comment """OPC: Each Tag has a Low Low Limit Parameter which acts as 
the Tag's Low Low Alarm Limit for evaluating alarm conditions from the Value Parameter.  
If the value of the Value Parameter exceeds the Low Low Limit the Tag is considered 
to be in a Low Low alarm condition."""@en ; 
    :opc-id 310 .

 :RCL   a rdf:Property ;
    rdfs:domain :Analog ;
    rdfs:range xsd:float ;
    rdfs:label "Rate of Change Limit"@en ; 
    rdfs:comment """OPC: Each Tag has a Rate of Change Limit Parameter which acts as 
the Tag's Rate of Change Alarm Limit for evaluating alarm conditions from the Value Parameter.  
If the value of the Value Parameter changes by more than the Units / Minute limit between samples 
that are sampled at the Sample Rate the Rate of Change Limit the Tag is considered to be in a ROC alarm condition."""@en ; 
    :opc-id 311 .

 :DL   a rdf:Property ;
    rdfs:domain :Analog ;
    rdfs:range xsd:float ;
    rdfs:label "Deviation Limit"@en ; 
    :opc-id 312 .

 :AlarmAreas a rdf:Property ;
    rdfs:range xsd:token ;
    rdfs:label "Alarm Area List"@en ; 
    rdfs:comment "OPC: An array of stings indicating the plant or alarm areas which include this ItemID."@en ; 
    :opc-id 302 .

 :PrimaryAlarmArea a rdf:Property ;
    rdfs:range xsd:token ;
    rdfs:label "Primary Alarm Area"@en ; 
    rdfs:comment "OPC: A string indicating the primary plant or alarm area including this ItemID"@en ; 
    :opc-id 303 .

 :ConditionLogic a rdf:Property ;
    rdfs:range xsd:string ;
    rdfs:label "Condition Logic"@en ; 
    rdfs:comment """OPC: An arbitrary string describing the test being performed. 
e.g. "High Limit Exceeded" or "TAG.PV >= TAG.HILIM" """@en ; 
    :opc-id 304 .

 :LimitExceeded a rdf:Property ;
    rdfs:range xsd:string ;
    rdfs:label "Limit Exceeded"@en ; 
    rdfs:comment "OPC: For multistate alarms, the condition exceeded e.g. HIHI, HI, LO, LOLO"@en ; 
    :opc-id 305 .

 :SoundFile a rdf:Property ;
    rdfs:range xsd:anyURI ;
    rdfs:label "Sound File"@en ; 
    :opc-id 313 .

#FIXME it's functional property: >mof:array/mof:tick
# :SSR a rdf:Property ;
#    rdfs:domain :ProcessPoint ;
#    rdfs:range xsd:int ;
#    rdfs:label "Частота обновления"@ru ;
#    rdfs:comment "Частота обновления в секундах"@ru .
